FSM.thy
@@ -323,6 +323,25 @@ definition language :: "('in, 'out, 'state) FSM \<Rightarrow> ('in * 'out) list 
 abbreviation L :: "('in, 'out, 'state) FSM \<Rightarrow> ('in * 'out) list set" where
 "L M \<equiv> language M"
 
+definition language_state_i :: "('in, 'out, 'state) FSM \<Rightarrow> 'state \<Rightarrow> 'in list \<Rightarrow> ('in * 'out) list set" where
+"language_state_i M s in_seq = { io . io \<in> language_state M s \<and> in_seq = map fst io }"
+
+lemma language_state_i_length :
+  assumes io: "io \<in> language_state_i M s iseq"
+  shows "length io = length iseq"
+proof -
+  have "iseq = map fst io" using io by (simp add: language_state_i_def)
+  then show ?thesis by simp
+qed
+
+lemma language_state_i_nil : "language_state_i M s [] = {Nil}"
+proof -
+  have "is_enabled_sequence M s []" by simp
+  then have nil_el : "Nil \<in> language_state M s" using get_io.simps(1) language_state_def by (metis (mono_tags, lifting) mem_Collect_eq)
+  have "\<forall> io \<in> language_state_i M s [] . length io = 0" by (simp add: language_state_i_def)
+  then have "language_state_i M s [] \<subseteq> {Nil}" by auto
+  then show ?thesis using nil_el using language_state_i_def by fastforce
+qed
 
 definition io_reduction_state :: "('in, 'out, 'state) FSM \<Rightarrow> 'state \<Rightarrow> ('in, 'out, 'state) FSM \<Rightarrow> 'state \<Rightarrow> bool" 
 where "io_reduction_state M1 s1 M2 s2 \<equiv> language_state M1 s1 \<subseteq> language_state M2 s2"
@@ -422,5 +441,7 @@ definition is_state_cover :: "('in, 'out, 'state) FSM \<Rightarrow> ('in * 'out)
   \<and> (\<forall> V2 . (V2 \<subset> V \<longrightarrow> (\<exists> s \<in> states M . d_reachable M s \<and> \<not> (\<exists> seq \<in> V . d_reaches M seq s))))
   (* contains Nil to reach (initial M) *)
   \<and> Nil \<in> V"
-  
+
+
+
 end
